---
layout: post
title:  "Porblem of the Week - Nov. 2, 2023 [Middle]"
date:   2023-11-02 00:12:00 -0700
tags: potw algebra
comments: "true"
inlinecomments: "true"
mathjax: "true"
publish_hint: "true"
publish_solution: "true"
publish_readmore: "true"
permalink: "potw/:title"
---
### Problem

Given $(x+\sqrt{x^2+2008})(y+\sqrt{y^2+2008})=2008$ï¼Œfind the value of $\dfrac{x+y}{x^2+y^2}$.

<!--more-->
<!-- https://zhuanlan.zhihu.com/p/74450871 -->

### Hint
{% if page.publish_hint == "true" or jekyll.environment == "preview" %}
- Irrational conjugates of $a+b\sqrt{c}$ is $a-b\sqrt{c}$. We can get their product quickly with the difference of two squares formula, saying $x^2-y^2=(x+y)(x-y)$
- A trick to deal with irrational expression is represent it as a new variable (e.g.: let $u=x+\sqrt{x^2+2008}$), then represent $x$ by $u$.

{% else %}
- to be published on 11/04/23.
{% endif %}

### Solution
{% if page.publish_solution == "true" or jekyll.environment == "preview" %}

**Solution 1:**

Let $u=x+\sqrt{x^2+2008}$, we have $(u-x)^2=x^2+2008$. Expand the left side, cancel the $x^2$ on both side, we have $u^2-2ux=2008$.

Similarly, let $v=y+\sqrt{y^2+2008}$, we have $v^2-2vy=2008$.

We also have $uv=2008$ given from the problem. Subsititue the $v=\dfrac{2008}{u}$ to $v^2-2vy=2008$, with some simplification, we can get $u^2+2uy=2008$.

Therefore, $x = -y$, $x+y=0$, and $\dfrac{x+y}{x^2+y^2}=0$.

**Solution 2:**

Considering the irrational conjugates of $x+\sqrt{x^2+2008}$, we have $(x+\sqrt{x^2+2008})(x-\sqrt{x^2+2008})=-2008$.

Let's rewrite the the given expression as $(\sqrt{x^2+2008}+x)(\sqrt{y^2+2008}+y)=2008$.

We also know $(\sqrt{x^2+2008}+x)(\sqrt{x^2+2008}-x)=2008$.

So, $\sqrt{y^2+2008}+y = \sqrt{x^2+2008}-x$

The above can be rewritten as $\sqrt{y^2+2008}+y = \sqrt{(-x)^2+2008}+(-x)$. It is straight forward to get y = -x.

Therefore, $x+y=0$, and $\dfrac{x+y}{x^2+y^2}=0$.


{% else %}
- to be published on 11/05/23.
{% endif %}

### Exercise Problem

### Read More
{% if page.publish_readmore == "true" or jekyll.environment == "preview" %}
- Provided that $a$ is a real number, solve equation $\sqrt{x+\sqrt{2x-1}} + \sqrt{x-\sqrt{2x-1}}=a$

{% else %}
- to be published on 11/02/23.
{% endif %}
